Clap/eDSLState/Varstore.lean
@@ -37,4 +37,10 @@ lemma subset_insert {p} {Γ : VarStore p} {k} {v} {h : k ∉ Γ}:
 := by
   aesop (add simp hasSubset_def) (add safe (by grind))
 
+@[grind =]
+lemma mem_iff_mem_keys {p} {Γ : VarStore p} {k}:
+  k ∈ Γ ↔ k ∈ Γ.keys
+:= by
+  grind
+
 end Clap.VarStore
